Change same_head to include permissions + add inject_unchanged_compose

backend/Mach2Mach2.v
@@ -21,24 +21,25 @@ Section WITHEXTCALLS.
 Section WITHINITSP.
   Variables init_ra: val.
   Variable return_address_offset: function -> code -> ptrofs -> Prop.
-  Variable ge: genv.
+  Variable prog: program.
+  Let ge:= Genv.globalenv prog.
 
   Inductive match_states : state -> state -> Prop :=
   | match_states_regular s f sp c rs m m'
                          (UNCH: Mem.unchanged_on (fun _ _ => True) m m')
-                         (SH: same_head (Mem.stack_adt m) (Mem.stack_adt m'))
+                         (SH: same_head (Mem.perm m) (Mem.stack_adt m) (Mem.stack_adt m'))
                          (NONIL: Forall (fun tf => tf <> nil) (Mem.stack_adt m'))
                          (NB: Mem.nextblock m = Mem.nextblock m'):
       match_states (State s f sp c rs m) (State s f sp c rs m')
   | match_states_call s fb rs m m'
                       (UNCH: Mem.unchanged_on (fun _ _ => True) m m')
-                      (SH: same_head ( (Mem.stack_adt m)) ( (Mem.stack_adt m')))
+                      (SH: same_head (Mem.perm m) (Mem.stack_adt m) (Mem.stack_adt m'))
                       (NONIL: Forall (fun tf => tf <> nil) (tl (Mem.stack_adt m')))
                       (NB: Mem.nextblock m = Mem.nextblock m'):
       match_states (Callstate s fb rs m) (Callstate s fb rs m')
   | match_states_return s rs m m'
                         (UNCH: Mem.unchanged_on (fun _ _ => True) m m')
-                        (SH: same_head ( (Mem.stack_adt m)) ( (Mem.stack_adt m')))
+                        (SH: same_head (Mem.perm m) (Mem.stack_adt m) (Mem.stack_adt m'))
                         (NONIL: Forall (fun tf => tf <> nil) (tl (Mem.stack_adt m')))
                         (NB: Mem.nextblock m = Mem.nextblock m'):
       match_states (Returnstate s rs m) (Returnstate s rs m').
@@ -68,15 +69,14 @@ Section WITHINITSP.
 
 
   Lemma storev_unchanged_on_1:
-    forall P chunk m m' addr v m1
-      (UNCH: Mem.unchanged_on P m m')
-      (SH: same_head (Mem.stack_adt m) (Mem.stack_adt m')
+    forall chunk m m' addr v m1
+      (UNCH: Mem.unchanged_on (fun _ _ => True) m m')
+      (SH: same_head (Mem.perm m) (Mem.stack_adt m) (Mem.stack_adt m')
            \/ forall b o, addr = Vptr b o -> ~ in_stack (Mem.stack_adt m') b
       )
-      (PERMALL: forall b o, P b o)
       (STORE: Mem.storev chunk m addr v = Some m1),
     exists m1',
-      Mem.storev chunk m' addr v = Some m1' /\ Mem.unchanged_on P m1 m1'.
+      Mem.storev chunk m' addr v = Some m1' /\ Mem.unchanged_on (fun _ _ => True) m1 m1'.
   Proof.
     destruct addr; simpl; intros; try congruence.
     eapply Mem.store_unchanged_on_1; eauto.
@@ -85,20 +85,18 @@ Section WITHINITSP.
   Qed.
 
   Lemma storestack_unchanged_on:
-    forall P m m' sp ty ofs v m1
-      (SH: same_head (Mem.stack_adt m) (Mem.stack_adt m') \/ forall b o, sp = Vptr b o -> ~ in_stack (Mem.stack_adt m') b)
-      (UNCH: Mem.unchanged_on P m m')
-      (Ptrue: forall b o, P b o)
+    forall m m' sp ty ofs v m1
+      (SH: same_head (Mem.perm m) (Mem.stack_adt m) (Mem.stack_adt m') \/ forall b o, sp = Vptr b o -> ~ in_stack (Mem.stack_adt m') b)
+      (UNCH: Mem.unchanged_on (fun _ _ => True) m m')
       (STORESTACK: store_stack m sp ty ofs v = Some m1),
     exists m1',
-      store_stack m' sp ty ofs v = Some m1' /\ Mem.unchanged_on P m1 m1'.
+      store_stack m' sp ty ofs v = Some m1' /\ Mem.unchanged_on (fun _ _ => True) m1 m1'.
   Proof.
     intros.
     unfold store_stack in *.
     eapply storev_unchanged_on_1; eauto.
     destruct SH;[left|right]; auto. intros; destruct sp; simpl in *; try congruence. inv H0. eapply H; eauto.
   Qed.
-
 
   Lemma eval_condition_unchanged:
     forall cond args m1 m2,
@@ -111,7 +109,6 @@ Section WITHINITSP.
     unfold eval_condition.
     repeat destr.
   Qed.
-
 
   Lemma eval_operation_unchanged:
     forall sp op args m1 m2,
@@ -195,8 +192,8 @@ Section WITHINITSP.
   Variable init_stk: stack_adt.
 
   Lemma parent_sp_same:
-    forall s1 s2
-      (SH: same_head s1 s2)
+    forall P s1 s2
+      (SH: same_head P s1 s2)
       (NONIL: Forall (fun tf => tf <> nil) (tl s2)),
       parent_sp s1 = parent_sp s2.
   Proof.
@@ -204,6 +201,20 @@ Section WITHINITSP.
     inv H0. auto. inv NONIL.
     repeat destr_in H1. auto.
   Qed.
+Lemma zle_zlt_false:
+  forall lo hi o,
+    zle lo o && zlt o hi = false <-> ~ (lo <= o < hi)%Z.
+Proof.
+  intros.
+  destruct (zle lo o), (zlt o hi); intuition; try congruence; try omega.
+Qed.
+
+Hypothesis frame_correct:
+  forall (fb : block) (f : function),
+    Genv.find_funct_ptr (Genv.globalenv prog) fb = Some (Internal f) ->
+    frame_size (fn_frame f) = fn_stacksize f.
+
+Existing Instance inject_perm_all.
 
   Lemma step_correct:
     forall S1 t S2 (STEP: Mach.step init_ra return_address_offset ge S1 t S2)
@@ -219,6 +230,7 @@ Section WITHINITSP.
     - edestruct storev_unchanged_on_1 as (m1' & STORE' & UNCH'); eauto. simpl; auto.
       eexists; split. econstructor; eauto.
       constructor; auto; repeat rewrite_stack_blocks; rewnb; auto.
+      eapply same_head_more_perm; eauto. intros b o k p INS. rewrite_perms. auto.
     - eexists; split. econstructor; eauto. eapply loadstack_unchanged_on; simpl; eauto. simpl. auto.
       erewrite <- parent_sp_same; eauto.
       apply Forall_tl; auto.
@@ -228,9 +240,11 @@ Section WITHINITSP.
     - eexists; split; econstructor; eauto. eapply loadv_unchanged_on; eauto. simpl; auto.
     - edestruct storev_unchanged_on_1 as (m1' & STORE' & UNCH'); eauto. simpl; auto.
       eexists; split; econstructor; eauto; repeat rewrite_stack_blocks; rewnb; auto.
+      eapply same_head_more_perm; eauto. intros b o k p INS. rewrite_perms. auto.
     - eexists; split; econstructor; eauto; repeat rewrite_stack_blocks; rewnb; auto.
       apply Mem.push_new_stage_strong_unchanged_on. auto.
       repeat rewrite_stack_blocks. constructor; auto.
+      eapply same_head_more_perm; eauto. intros b o k p INS. rewrite_perms. auto.
     - edestruct Mem.unchanged_on_free as (m2' & FREE' & UNCH'); eauto.
       inv CSC. rewrite FIND in H0; inv H0.
       edestruct (clear_stage_unchanged _ _ UNCH') as (m3' & USB & UNCH'').
@@ -238,12 +252,40 @@ Section WITHINITSP.
       eexists; split; econstructor; eauto. eapply loadstack_unchanged_on; eauto. simpl; auto.
       repeat rewrite_stack_blocks; auto.
       inv CallStackConsistency. rewrite <- H6 in SH. inv SH. simpl. constructor; auto.
-      destr.
+      {
+        split. destr.
+        intros. destruct H5. destr_in H5. subst.
+        exfalso.
+        assert (f1 = f0).
+        destruct H3; auto.
+        destruct H4 as (b & o & k & p & NONE & IFR & PERMS & IPC).                 
+        exploit Mem.wf_stack_mem. rewrite <- H0.
+        intro A; inv A.
+        red in H9; simpl in H9. exfalso.
+        eapply in_frame_in_frames in IFR; eauto.
+        revert PERMS. rewrite_perms. destr. intros.
+        eapply (H9 b); eauto. subst.
+        destruct H4 as (b & o & k & p & NONE & IFR & PERMS & IPC).
+        revert PERMS. rewrite_perms.
+        unfold in_frame, get_frame_blocks in IFR. rewrite BLOCKS in IFR. destruct IFR as [IFR|[]].
+        inv IFR. simpl in *.
+        rewrite Ptrofs.unsigned_zero. simpl.
+        destr. rewrite <- andb_assoc in Heqb. rewrite andb_false_iff in Heqb.
+        destruct Heqb. contradict H4. destruct peq; simpl; auto. congruence.
+        apply zle_zlt_false in H4. intro.
+        exploit Mem.agree_perms_mem. rewrite <- H0. left. reflexivity. left. reflexivity.
+        rewrite BLOCKS.
+        left; reflexivity. apply H5. erewrite frame_correct; eauto.
+      }
+      eapply same_head_more_perm. apply H7. intros b o k p H3.
+      rewrite_perms. destr.
       repeat  rewrite_stack_blocks; simpl; auto. inv NONIL; auto; constructor.
       rewnb. auto.
     - edestruct ec_unchanged_on as (m2' & EXTCALL & UNCH' & NB'). apply external_call_spec. 4: eauto.
       apply Mem.push_new_stage_strong_unchanged_on. eauto.
-      repeat rewrite_stack_blocks. constructor. auto. auto.
+      repeat rewrite_stack_blocks. constructor. split; auto.
+      eapply same_head_more_perm. apply SH.
+      intros b0 o k p H2. rewrite_perms. auto.
       rewnb. auto.
       edestruct Mem.unchanged_on_unrecord as (m3' & USB & UNCH''). apply UNCH'.
       eapply list_forall2_length. eauto.
@@ -251,7 +293,9 @@ Section WITHINITSP.
       eauto.
       eexists; split; econstructor; eauto.
       eapply unchanged_on_builtin_args; eauto.
-      repeat rewrite_stack_blocks; eauto.
+      repeat rewrite_stack_blocks; simpl; eauto.
+      eapply same_head_more_perm; eauto. intros b0 o k p H2.
+      repeat rewrite_perms. auto. rewrite_stack_blocks. simpl; auto.
       repeat rewrite_stack_blocks; eauto.
       rewnb; auto.
     - eexists; split; econstructor; eauto.
@@ -267,7 +311,34 @@ Section WITHINITSP.
       rewrite_stack_blocks. inv CallStackConsistency. simpl; omega.
       eexists; split; econstructor; eauto. eapply loadstack_unchanged_on; eauto. simpl; auto.
       repeat rewrite_stack_blocks; auto. simpl.
-      inv CallStackConsistency. rewrite <- H in SH. inv SH. constructor; simpl; auto. destr.
+      inv CallStackConsistency. rewrite <- H in SH. inv SH. constructor; simpl; auto.
+      {
+        split. destr.
+        intros. destruct H5. destr_in H5. subst.
+        exfalso.
+        assert (f1 = f0).
+        destruct H3; auto.
+        destruct H4 as (b & o & k & p & NONE & IFR & PERMS & IPC).                 
+        exploit Mem.wf_stack_mem. rewrite <- H2.
+        intro A; inv A.
+        red in H8; simpl in H8. exfalso.
+        eapply in_frame_in_frames in IFR; eauto.
+        revert PERMS. rewrite_perms. destr. intros.
+        eapply (H8 b); eauto. subst.
+        destruct H4 as (b & o & k & p & NONE & IFR & PERMS & IPC).
+        revert PERMS. rewrite_perms.
+        unfold in_frame, get_frame_blocks in IFR. rewrite BLOCKS in IFR. destruct IFR as [IFR|[]].
+        inv IFR. simpl in *.
+        rewrite Ptrofs.unsigned_zero. simpl.
+        destr. rewrite <- andb_assoc in Heqb. rewrite andb_false_iff in Heqb.
+        destruct Heqb. contradict H4. destruct peq; simpl; auto. congruence.
+        apply zle_zlt_false in H4. intro.
+        exploit Mem.agree_perms_mem. rewrite <- H2. left. reflexivity. left. reflexivity.
+        rewrite BLOCKS.
+        left; reflexivity. apply H5. erewrite frame_correct; eauto.
+      }
+      eapply same_head_more_perm. apply H6. intros b o k p H3.
+      rewrite_perms. destr.
       repeat rewrite_stack_blocks; auto. simpl. apply Forall_tl; auto.
       rewnb. auto.
     - destruct (Mem.alloc m' 0 (fn_stacksize f)) as (m1' & stk') eqn:ALLOC.
@@ -275,17 +346,34 @@ Section WITHINITSP.
       apply Mem.alloc_result in ALLOC.
       apply Mem.alloc_result in H1. congruence. subst.
       generalize (Mem.unchanged_on_alloc _ _ UNCH _ _ _ _ H1 _ ALLOC). intro UNCH1.
-      edestruct (fun SH => storestack_unchanged_on _ _ _ _ _ _ _ _ SH UNCH1 (fun _ _ => I) H2) as (m3' & STORE & UNCH2).
+      edestruct (fun SH => storestack_unchanged_on _ _ _ _ _ _ _ SH UNCH1 H2) as (m3' & STORE & UNCH2).
       repeat rewrite_stack_blocks. right; intro; subst. inversion 1; subst.
       intro INS. subst. eapply Mem.fresh_block_alloc; eauto. eapply Mem.in_frames_valid; eauto.
       edestruct (Mem.unchanged_on_record) as (m5' & RSB & UNCH4).
       4: apply H3. eauto. unfold store_stack in *. rewnb. congruence.
       unfold store_stack in *; repeat rewrite_stack_blocks; auto.
+      eapply same_head_more_perm; eauto.
+      intros b o k p H4. repeat rewrite_perms. destr. subst.
+      exfalso. eapply Mem.in_frames_valid in H4. eapply Mem.fresh_block_alloc in H4; eauto.
       eexists; split; econstructor; eauto.
       unfold store_stack in *; repeat rewrite_stack_blocks.
       revert EQ1 EQ0; repeat rewrite_stack_blocks. intros A B; rewrite A, B in SH.
       inv CSC. red in TIN. rewrite B in TIN. inv TIN.
       inv SH. constructor; auto.
+      split; auto.
+      {
+        simpl. intros f1 [AA|AA]; auto. intros (bb & o & k & p & NONE & IFR & PERM & _).
+        exfalso.
+        exploit Mem.wf_stack_mem. rewrite EQ2.
+        intro WF; inv WF.
+        red in H6; simpl in H6. exfalso.
+        eapply in_frame_in_frames in IFR; eauto.
+        eapply (H6 bb); eauto.        
+      }
+      eapply same_head_more_perm; eauto.
+      intros b o k p H4. repeat rewrite_perms. destr. subst.
+      exploit Mem.in_frames_valid. rewrite A. rewrite in_stack_cons. right. eauto.
+      intro VB. exfalso; eapply Mem.fresh_block_alloc in VB; eauto.
       unfold store_stack in *.
       repeat rewrite_stack_blocks. revert EQ1; repeat rewrite_stack_blocks. intro EQ1; rewrite EQ1 in NONIL.
       simpl in NONIL. constructor; auto. congruence.
@@ -296,12 +384,16 @@ Section WITHINITSP.
       erewrite <- parent_sp_same; eauto.
       eapply unchanged_on_extcall_args; eauto.
       repeat rewrite_stack_blocks; eauto.
+      eapply same_head_more_perm; eauto. intros b0 o k p H2.
+      repeat rewrite_perms. auto. auto.
       repeat rewrite_stack_blocks; eauto.
     - edestruct Mem.unchanged_on_unrecord as (m1' & USB & UNCH''). apply UNCH.
       eapply list_forall2_length; eauto.
       eauto.
       eexists; split; econstructor; eauto.
       repeat rewrite_stack_blocks; eauto. inv SH; auto. constructor.
+      eapply same_head_more_perm. simpl. apply H3. simpl.
+      intros b o k p H4. rewrite_perms. auto.
       repeat rewrite_stack_blocks; eauto.
       rewnb; auto.
   Qed.
@@ -315,8 +407,9 @@ End WITHINITSP.
     intros p s IS. inv IS.
     constructor; try reflexivity.
     - apply Mem.unchanged_on_refl.
-    - repeat rewrite_stack_blocks. simpl.
+    - repeat rewrite_stack_blocks.
       repeat constructor; auto.
+      destr_in H3; auto. easy.
     - repeat rewrite_stack_blocks. simpl. repeat constructor. congruence.
   Qed.
 
